wip: exp_fw

code/bignum/Hacl.Spec.Exponentiation.Lemmas.fst
@@ -107,18 +107,18 @@ let rec pow_nat_mont_is_pow n r d aM b =
       }; () end
 
 
-val mont_mod_exp: n:pos -> r:pos -> d:int{r * d % n == 1} -> a:nat_mod n -> b:pos -> nat_mod n
-let mont_mod_exp n r d a b =
+val mod_exp_mont: n:pos -> r:pos -> d:int{r * d % n == 1} -> a:nat_mod n -> b:pos -> nat_mod n
+let mod_exp_mont n r d a b =
   let aM = a * r % n in
   let accM = LE.pow (mk_nat_mont_group n r d) aM b in
   let acc = accM * d % n in
   acc
 
 
-val mont_mod_exp_lemma_before_to_mont: n:pos -> r:pos -> d:int{r * d % n == 1} -> a:nat_mod n -> b:pos ->
+val mod_exp_mont_lemma_before_to_mont: n:pos -> r:pos -> d:int{r * d % n == 1} -> a:nat_mod n -> b:pos ->
   Lemma (pow (a * r % n) b * oneM n r * pow d b % n == pow a b * oneM n r % n)
 
-let mont_mod_exp_lemma_before_to_mont n r d a b =
+let mod_exp_mont_lemma_before_to_mont n r d a b =
   let aM = a * r % n in
   let accM0 = oneM n r in
   calc (==) {
@@ -142,10 +142,10 @@ let mont_mod_exp_lemma_before_to_mont n r d a b =
   assert (pow aM b * accM0 * pow d b % n == pow a b * accM0 % n)
 
 
-val mont_mod_exp_lemma_after_to_mont: n:pos -> r:pos -> d:int{r * d % n == 1} -> a:nat_mod n -> b:pos ->
+val mod_exp_mont_lemma_after_to_mont: n:pos -> r:pos -> d:int{r * d % n == 1} -> a:nat_mod n -> b:pos ->
   Lemma (pow a b * oneM n r % n * d % n == pow a b % n)
 
-let mont_mod_exp_lemma_after_to_mont n r d a b =
+let mod_exp_mont_lemma_after_to_mont n r d a b =
   let accM0 = oneM n r in
   calc (==) {
     pow a b * accM0 % n * d % n;
@@ -162,19 +162,19 @@ let mont_mod_exp_lemma_after_to_mont n r d a b =
   }
 
 
-val mont_mod_exp_lemma: n:pos -> r:pos -> d:int{r * d % n == 1} -> a:nat_mod n -> b:pos ->
-  Lemma (mont_mod_exp n r d a b == pow a b % n)
+val mod_exp_mont_lemma: n:pos -> r:pos -> d:int{r * d % n == 1} -> a:nat_mod n -> b:pos ->
+  Lemma (mod_exp_mont n r d a b == pow a b % n)
 
-let mont_mod_exp_lemma n r d a b =
+let mod_exp_mont_lemma n r d a b =
   let k = mk_nat_mont_group n r d in
   let aM = a * r % n in
   calc (==) {
     LE.pow k aM b * d % n;
     (==) { pow_nat_mont_is_pow n r d aM b }
     pow aM b * oneM n r * pow d b % n * d % n;
-    (==) { mont_mod_exp_lemma_before_to_mont n r d a b }
+    (==) { mod_exp_mont_lemma_before_to_mont n r d a b }
     pow a b * oneM n r % n * d % n;
-    (==) { mont_mod_exp_lemma_after_to_mont n r d a b }
+    (==) { mod_exp_mont_lemma_after_to_mont n r d a b }
     pow a b % n;
     }
 
@@ -289,36 +289,77 @@ let rec pow_nat_mont_ll_is_pow_nat_mont pbits rLen n mu a b =
     () end
 
 
+val mod_exp_mont_ll: pbits:pos -> rLen:pos -> n:pos -> mu:nat{mont_pre pbits rLen n mu}
+  -> a:nat_mod n -> b:pos -> nat_mod n
+
+let mod_exp_mont_ll pbits rLen n mu a b =
+  let d, k = M.eea_pow2_odd (pbits * rLen) n in
+  M.mont_preconditions_d pbits rLen n;
+
+  let aM = M.to_mont pbits rLen n mu a in
+  M.to_mont_lemma pbits rLen n d mu a;
+  let accM = LE.pow (mk_nat_mont_group_ll pbits rLen n mu) aM b in
+  let acc = M.from_mont pbits rLen n mu accM in
+  M.from_mont_lemma pbits rLen n d mu accM;
+  acc
+
+
+val mod_exp_mont_ll_lemma: pbits:pos -> rLen:pos -> n:pos -> mu:nat{mont_pre pbits rLen n mu}
+  -> a:nat_mod n -> b:pos ->
+  Lemma (mod_exp_mont_ll pbits rLen n mu a b == pow a b % n)
+
+let mod_exp_mont_ll_lemma pbits rLen n mu a b =
+  let r = pow2 (pbits * rLen) in
+  let d, k = M.eea_pow2_odd (pbits * rLen) n in
+  M.mont_preconditions_d pbits rLen n;
+
+  let k1 = mk_nat_mont_group_ll pbits rLen n mu in
+  let k2 = mk_nat_mont_group n r d in
+
+  let aM = M.to_mont pbits rLen n mu a in
+  M.to_mont_lemma pbits rLen n d mu a;
+  assert (aM == a * r % n);
+
+  let accM = LE.pow k1 aM b in
+  pow_nat_mont_ll_is_pow_nat_mont pbits rLen n mu aM b;
+  assert (accM == LE.pow k2 aM b);
+
+  let acc = M.from_mont pbits rLen n mu accM in
+  M.from_mont_lemma pbits rLen n d mu accM;
+  assert (acc == accM * d % n);
+  mod_exp_mont_lemma n r d a b
+
+
 ///  A righ-to-left binary method with Montgomery arithmetic
 ///  using functions defined in Hacl.Spec.Montgomery.Lemmas
 
-val mod_exp_mont_f_ll:
+val mod_exp_rl_mont_f:
     pbits:pos -> rLen:nat
   -> n:pos -> mu:nat
   -> bBits:nat -> b:nat{b < pow2 bBits}
   -> i:nat{i < bBits} -> tuple2 nat nat ->
   tuple2 nat nat
 
-let mod_exp_mont_f_ll pbits rLen n mu bBits b i (aM, accM) =
+let mod_exp_rl_mont_f pbits rLen n mu bBits b i (aM, accM) =
   let accM = if (b / pow2 i % 2 = 1) then M.mont_mul pbits rLen n mu accM aM else accM in
   let aM = M.mont_mul pbits rLen n mu aM aM in
   (aM, accM)
 
 
-val mod_exp_mont_ll:
+val mod_exp_rl_mont:
     pbits:pos -> rLen:nat
   -> n:pos -> mu:nat
   -> a:nat -> bBits:nat -> b:pos{b < pow2 bBits} ->
   nat
 
-let mod_exp_mont_ll pbits rLen n mu a bBits b =
+let mod_exp_rl_mont pbits rLen n mu a bBits b =
   let aM = M.to_mont pbits rLen n mu a in
   let accM = M.to_mont pbits rLen n mu 1 in
-  let (aM, accM) = Loops.repeati bBits (mod_exp_mont_f_ll pbits rLen n mu bBits b) (aM, accM) in
+  let (aM, accM) = Loops.repeati bBits (mod_exp_rl_mont_f pbits rLen n mu bBits b) (aM, accM) in
   M.from_mont pbits rLen n mu accM
 
 
-val mod_exp_mont_ll_lemma_loop:
+val mod_exp_rl_mont_lemma_loop:
     pbits:pos -> rLen:nat
   -> n:pos -> mu:nat
   -> bBits:nat -> b:pos{b < pow2 bBits}
@@ -327,36 +368,34 @@ val mod_exp_mont_ll_lemma_loop:
   (requires mont_pre pbits rLen n mu)
   (ensures
    (let k = mk_nat_mont_group_ll pbits rLen n mu in
-    let aM1, accM1 = Loops.repeati i (mod_exp_mont_f_ll pbits rLen n mu bBits b) (aM0, accM0) in
+    let aM1, accM1 = Loops.repeati i (mod_exp_rl_mont_f pbits rLen n mu bBits b) (aM0, accM0) in
     let aM2, accM2 = Loops.repeati i (LE.exp_rl_f k bBits b) (aM0, accM0) in
     aM1 == aM2 /\ accM1 == accM2))
 
-let rec mod_exp_mont_ll_lemma_loop pbits rLen n mu bBits b i aM0 accM0 =
+let rec mod_exp_rl_mont_lemma_loop pbits rLen n mu bBits b i aM0 accM0 =
   let k = mk_nat_mont_group_ll pbits rLen n mu in
 
   if i = 0 then begin
-    Loops.eq_repeati0 i (mod_exp_mont_f_ll pbits rLen n mu bBits b) (aM0, accM0);
+    Loops.eq_repeati0 i (mod_exp_rl_mont_f pbits rLen n mu bBits b) (aM0, accM0);
     Loops.eq_repeati0 i (LE.exp_rl_f k bBits b) (aM0, accM0) end
   else begin
-    Loops.unfold_repeati i (mod_exp_mont_f_ll pbits rLen n mu bBits b) (aM0, accM0) (i - 1);
+    Loops.unfold_repeati i (mod_exp_rl_mont_f pbits rLen n mu bBits b) (aM0, accM0) (i - 1);
     Loops.unfold_repeati i (LE.exp_rl_f k bBits b) (aM0, accM0) (i - 1);
-    mod_exp_mont_ll_lemma_loop pbits rLen n mu bBits b (i - 1) aM0 accM0 end
+    mod_exp_rl_mont_lemma_loop pbits rLen n mu bBits b (i - 1) aM0 accM0 end
 
 
-val mod_exp_mont_ll_lemma:
+val mod_exp_rl_mont_lemma:
     pbits:pos -> rLen:nat
   -> n:pos -> mu:nat
   -> a:nat_mod n
   -> bBits:nat -> b:pos{b < pow2 bBits} -> Lemma
   (requires mont_pre pbits rLen n mu)
-  (ensures  mod_exp_mont_ll pbits rLen n mu a bBits b == pow_mod #n a b)
+  (ensures  mod_exp_rl_mont pbits rLen n mu a bBits b == pow_mod #n a b)
 
-let mod_exp_mont_ll_lemma pbits rLen n mu a bBits b =
+let mod_exp_rl_mont_lemma pbits rLen n mu a bBits b =
   let r = pow2 (pbits * rLen) in
   let d, k = M.eea_pow2_odd (pbits * rLen) n in
   M.mont_preconditions_d pbits rLen n;
-
-  let k0 = mk_nat_mont_group n r d in
   let k1 = mk_nat_mont_group_ll pbits rLen n mu in
 
   let aM0 = M.to_mont pbits rLen n mu a in
@@ -366,29 +405,28 @@ let mod_exp_mont_ll_lemma pbits rLen n mu a bBits b =
   assert (aM0 == a * r % n);
   assert (accM0 == 1 * r % n);
 
-  let (aM1, accM1) = Loops.repeati bBits (mod_exp_mont_f_ll pbits rLen n mu bBits b) (aM0, accM0) in
-  mod_exp_mont_ll_lemma_loop pbits rLen n mu bBits b bBits aM0 accM0;
+  let (aM1, accM1) = Loops.repeati bBits (mod_exp_rl_mont_f pbits rLen n mu bBits b) (aM0, accM0) in
+  mod_exp_rl_mont_lemma_loop pbits rLen n mu bBits b bBits aM0 accM0;
   LE.exp_rl_lemma k1 aM0 bBits b;
-  //assert (accM1 == LE.pow k1 aM0 b);
-  pow_nat_mont_ll_is_pow_nat_mont pbits rLen n mu aM0 b;
-  //assert (accM1 == LE.pow k0 aM0 b);
+  assert (accM1 == LE.pow k1 aM0 b);
   let res = M.from_mont pbits rLen n mu accM1 in
   M.from_mont_lemma pbits rLen n d mu accM1;
-  mont_mod_exp_lemma n r d a b;
+  mod_exp_mont_ll_lemma pbits rLen n mu a b;
+  assert (res == pow a b % n);
   lemma_pow_mod #n a b
 
 
 ///  Montgomery ladder for exponentiation with Montgomery arithmetic and
 ///  conditional swap using functions defined in Hacl.Spec.Montgomery.Lemmas
 
-val mod_exp_mont_ladder_swap_f_ll:
+val mod_exp_mont_ladder_swap_f:
     pbits:pos -> rLen:nat
   -> n:pos -> mu:nat
   -> bBits:nat -> b:nat{b < pow2 bBits}
   -> i:nat{i < bBits} -> tuple3 nat nat nat ->
   tuple3 nat nat nat
 
-let mod_exp_mont_ladder_swap_f_ll pbits rLen n mu bBits b i (rM0, rM1, privbit) =
+let mod_exp_mont_ladder_swap_f pbits rLen n mu bBits b i (rM0, rM1, privbit) =
   let bit = b / pow2 (bBits - i - 1) % 2 in
   let sw = (bit + privbit) % 2 in
   let rM0, rM1 = LE.cswap sw rM0 rM1 in
@@ -396,23 +434,23 @@ let mod_exp_mont_ladder_swap_f_ll pbits rLen n mu bBits b i (rM0, rM1, privbit) 
   (rM0, rM1, bit)
 
 
-val mod_exp_mont_ladder_swap_ll:
+val mod_exp_mont_ladder_swap:
     pbits:pos -> rLen:nat
   -> n:pos -> mu:nat
   -> a:nat -> bBits:nat -> b:nat{b < pow2 bBits} ->
   nat
 
-let mod_exp_mont_ladder_swap_ll pbits rLen n mu a bBits b =
+let mod_exp_mont_ladder_swap pbits rLen n mu a bBits b =
   let rM0 = M.to_mont pbits rLen n mu 1 in
   let rM1 = M.to_mont pbits rLen n mu a in
   let sw = 0 in
   let (rM0', rM1', sw') =
-    Loops.repeati bBits (mod_exp_mont_ladder_swap_f_ll pbits rLen n mu bBits b) (rM0, rM1, sw) in
+    Loops.repeati bBits (mod_exp_mont_ladder_swap_f pbits rLen n mu bBits b) (rM0, rM1, sw) in
   let rM0', rM1' = LE.cswap sw' rM0' rM1' in
   M.from_mont pbits rLen n mu rM0'
 
 
-val mod_exp_mont_lader_swap_ll_lemma_loop:
+val mod_exp_mont_lader_swap_lemma_loop:
     pbits:pos -> rLen:nat
   -> n:pos -> mu:nat
   -> bBits:nat -> b:pos{b < pow2 bBits}
@@ -424,36 +462,34 @@ val mod_exp_mont_lader_swap_ll_lemma_loop:
   (ensures
     (let k = mk_nat_mont_group_ll pbits rLen n mu in
      let (rM0', rM1', sw') = Loops.repeati i
-       (mod_exp_mont_ladder_swap_f_ll pbits rLen n mu bBits b) (rM0, rM1, sw0) in
+       (mod_exp_mont_ladder_swap_f pbits rLen n mu bBits b) (rM0, rM1, sw0) in
      let (rM0'', rM1'', sw'') = Loops.repeati i (LE.exp_mont_ladder_swap_f k bBits b) (rM0, rM1, sw0) in
      rM0' == rM0'' /\ rM1' == rM1'' /\ sw' == sw''))
 
-let rec mod_exp_mont_lader_swap_ll_lemma_loop pbits rLen n mu bBits b i rM0 rM1 sw0 =
+let rec mod_exp_mont_lader_swap_lemma_loop pbits rLen n mu bBits b i rM0 rM1 sw0 =
   let k = mk_nat_mont_group_ll pbits rLen n mu in
 
   if i = 0 then begin
-    Loops.eq_repeati0 i (mod_exp_mont_ladder_swap_f_ll pbits rLen n mu bBits b) (rM0, rM1, sw0);
+    Loops.eq_repeati0 i (mod_exp_mont_ladder_swap_f pbits rLen n mu bBits b) (rM0, rM1, sw0);
     Loops.eq_repeati0 i (LE.exp_mont_ladder_swap_f k bBits b) (rM0, rM1, sw0) end
   else begin
-    Loops.unfold_repeati i (mod_exp_mont_ladder_swap_f_ll pbits rLen n mu bBits b) (rM0, rM1, sw0) (i - 1);
+    Loops.unfold_repeati i (mod_exp_mont_ladder_swap_f pbits rLen n mu bBits b) (rM0, rM1, sw0) (i - 1);
     Loops.unfold_repeati i (LE.exp_mont_ladder_swap_f k bBits b) (rM0, rM1, sw0) (i - 1);
-    mod_exp_mont_lader_swap_ll_lemma_loop pbits rLen n mu bBits b (i - 1) rM0 rM1 sw0 end
+    mod_exp_mont_lader_swap_lemma_loop pbits rLen n mu bBits b (i - 1) rM0 rM1 sw0 end
 
 
-val mod_exp_mont_ladder_swap_ll_lemma:
+val mod_exp_mont_ladder_swap_lemma:
     pbits:pos -> rLen:nat
   -> n:pos -> mu:nat
   -> a:nat_mod n
   -> bBits:nat -> b:pos{b < pow2 bBits} -> Lemma
   (requires mont_pre pbits rLen n mu)
-  (ensures  mod_exp_mont_ladder_swap_ll pbits rLen n mu a bBits b == pow_mod #n a b)
+  (ensures  mod_exp_mont_ladder_swap pbits rLen n mu a bBits b == pow_mod #n a b)
 
-let mod_exp_mont_ladder_swap_ll_lemma pbits rLen n mu a bBits b =
+let mod_exp_mont_ladder_swap_lemma pbits rLen n mu a bBits b =
   let r = pow2 (pbits * rLen) in
   let d, k = M.eea_pow2_odd (pbits * rLen) n in
   M.mont_preconditions_d pbits rLen n;
-
-  let k0 = mk_nat_mont_group n r d in
   let k1 = mk_nat_mont_group_ll pbits rLen n mu in
 
   let rM0 = M.to_mont pbits rLen n mu 1 in
@@ -466,33 +502,33 @@ let mod_exp_mont_ladder_swap_ll_lemma pbits rLen n mu a bBits b =
   let sw0 = 0 in
   Math.Lemmas.small_div b (pow2 bBits);
   assert (sw0 == b / pow2 bBits % 2);
-  let (rM0', rM1', sw') = Loops.repeati bBits
-    (mod_exp_mont_ladder_swap_f_ll pbits rLen n mu bBits b) (rM0, rM1, sw0) in
+
+  let (rM0', rM1', sw') = Loops.repeati bBits (mod_exp_mont_ladder_swap_f pbits rLen n mu bBits b) (rM0, rM1, sw0) in
   let (rM0'', rM1'', sw'') = Loops.repeati bBits (LE.exp_mont_ladder_swap_f k1 bBits b) (rM0, rM1, sw0) in
-  mod_exp_mont_lader_swap_ll_lemma_loop pbits rLen n mu bBits b bBits rM0 rM1 sw0;
+  mod_exp_mont_lader_swap_lemma_loop pbits rLen n mu bBits b bBits rM0 rM1 sw0;
   assert (rM0' == rM0'' /\ rM1' == rM1'' /\ sw' == sw'');
 
   let rM0', rM1' = LE.cswap sw' rM0' rM1' in
   LE.exp_mont_ladder_swap_lemma k1 rM1 bBits b;
   LE.exp_mont_ladder_lemma k1 rM1 bBits b;
   assert (rM0' == LE.pow k1 rM1 b);
-  pow_nat_mont_ll_is_pow_nat_mont pbits rLen n mu rM1 b;
-  assert (rM0' == LE.pow k0 rM1 b);
 
+  let res = M.from_mont pbits rLen n mu rM0' in
   M.from_mont_lemma pbits rLen n d mu rM0';
-  mont_mod_exp_lemma n r d a b;
+  mod_exp_mont_ll_lemma pbits rLen n mu a b;
+  assert (res == pow a b % n);
   lemma_pow_mod #n a b
 
 ///  Fixed window exponentiation with a precomputed table and Montgomery arithmetic
 ///  using functions defined in Hacl.Spec.Montgomery.Lemmas
 
 // res == pow acc (pow2 b)
-val mod_exp_mont_pow2: pbits:pos -> rLen:nat -> n:pos -> mu:nat -> a:nat -> b:nat -> nat
-let mod_exp_mont_pow2 pbits rLen n mu a b =
+val mod_exp_pow2_mont: pbits:pos -> rLen:nat -> n:pos -> mu:nat -> a:nat -> b:nat -> nat
+let mod_exp_pow2_mont pbits rLen n mu a b =
   Loops.repeat b (M.mont_sqr pbits rLen n mu) a
 
 
-val mod_exp_mont_precomp_table_f:
+val mod_precomp_table_mont_f:
     pbits:pos -> rLen:nat
   -> n:pos -> mu:nat
   -> a:nat
@@ -501,27 +537,27 @@ val mod_exp_mont_precomp_table_f:
   -> table:lseq nat table_len ->
   lseq nat table_len
 
-let mod_exp_mont_precomp_table_f pbits rLen n mu a table_len i table =
+let mod_precomp_table_mont_f pbits rLen n mu a table_len i table =
   table.[i + 2] <- M.mont_mul pbits rLen n mu table.[i + 1] a
 
 // table_len = pow2 l
 // table.[i] == pow a i
-val mod_exp_mont_precomp_table:
+val mod_precomp_table_mont:
     pbits:pos -> rLen:nat
   -> n:pos -> mu:nat
   -> table_len:Lib.IntTypes.size_nat{1 < table_len}
   -> a:nat ->
   lseq nat table_len
 
-let mod_exp_mont_precomp_table pbits rLen n mu table_len a =
+let mod_precomp_table_mont pbits rLen n mu table_len a =
   let table = create table_len 0 in
   let table = table.[0] <- M.to_mont pbits rLen n mu 1 in
   let table = table.[1] <- a in
 
-  Loops.repeati (table_len - 2) (mod_exp_mont_precomp_table_f pbits rLen n mu a table_len) table
+  Loops.repeati (table_len - 2) (mod_precomp_table_mont_f pbits rLen n mu a table_len) table
 
 
-val mod_exp_mont_precomp_f_ll:
+val mod_exp_fw_mont_f:
     pbits:pos -> rLen:nat
   -> n:pos -> mu:nat
   -> bBits:nat -> b:nat{b < pow2 bBits}
@@ -531,14 +567,14 @@ val mod_exp_mont_precomp_f_ll:
   -> i:nat{l * (i + 1) <= bBits} -> acc:nat ->
   nat
 
-let mod_exp_mont_precomp_f_ll pbits rLen n mu bBits b l table_len table i acc =
+let mod_exp_fw_mont_f pbits rLen n mu bBits b l table_len table i acc =
   let bits_l = b / pow2 (bBits - l * i - l) % table_len in
-  let acc_pow2l = mod_exp_mont_pow2 pbits rLen n mu acc l in // pow k acc (pow2 l)
+  let acc_pow2l = mod_exp_pow2_mont pbits rLen n mu acc l in // pow k acc (pow2 l)
   let a_powbits_l = table.[bits_l] in //select_table // pow k a bits_l
   M.mont_mul pbits rLen n mu acc_pow2l a_powbits_l
 
 
-val mod_exp_mont_precomp_rem_ll:
+val mod_exp_fw_mont_rem:
     pbits:pos -> rLen:nat
   -> n:pos -> mu:nat
   -> bBits:nat -> b:nat{b < pow2 bBits}
@@ -547,16 +583,16 @@ val mod_exp_mont_precomp_rem_ll:
   -> table:lseq nat table_len -> accM:nat ->
   nat
 
-let mod_exp_mont_precomp_rem_ll pbits rLen n mu bBits b l table_len table accM =
+let mod_exp_fw_mont_rem pbits rLen n mu bBits b l table_len table accM =
   let c = bBits % l in
   let bits_c = b % pow2 c in
-  let acc_pow2c = mod_exp_mont_pow2 pbits rLen n mu accM c in // pow k acc (pow2 c)
+  let acc_pow2c = mod_exp_pow2_mont pbits rLen n mu accM c in // pow k acc (pow2 c)
   Math.Lemmas.pow2_lt_compat l c;
   let a_powbits_c = table.[bits_c] in //select_table // pow k a bits_c
   M.mont_mul pbits rLen n mu acc_pow2c a_powbits_c
 
 
-val mod_exp_mont_precomp_table_ll:
+val mod_exp_fw_mont_:
     pbits:pos -> rLen:nat
   -> n:pos -> mu:nat
   -> aM:nat
@@ -564,38 +600,40 @@ val mod_exp_mont_precomp_table_ll:
   -> l:pos{pow2 l <= Lib.IntTypes.max_size_t} ->
   nat
 
-let mod_exp_mont_precomp_table_ll pbits rLen n mu aM bBits b l =
+let mod_exp_fw_mont_ pbits rLen n mu aM bBits b l =
   let oneM = M.to_mont pbits rLen n mu 1 in
   let table_len = pow2 l in
   Math.Lemmas.pow2_le_compat l 1;
-  let table = mod_exp_mont_precomp_table pbits rLen n mu table_len aM in
-  let accM = Loops.repeati (bBits / l) (mod_exp_mont_precomp_f_ll pbits rLen n mu bBits b l table_len table) oneM in
-  mod_exp_mont_precomp_rem_ll pbits rLen n mu bBits b l table_len table accM
+  let table = mod_precomp_table_mont pbits rLen n mu table_len aM in
+  let accM = Loops.repeati (bBits / l) (mod_exp_fw_mont_f pbits rLen n mu bBits b l table_len table) oneM in
+  if bBits % l = 0 then accM else mod_exp_fw_mont_rem pbits rLen n mu bBits b l table_len table accM
 
 
-val mod_exp_mont_precomp_ll:
+val mod_exp_fw_mont:
     pbits:pos -> rLen:nat
   -> n:pos -> mu:nat
   -> a:nat -> bBits:nat -> b:nat{b < pow2 bBits}
   -> l:pos{pow2 l <= Lib.IntTypes.max_size_t} ->
   nat
 
-let mod_exp_mont_precomp_ll pbits rLen n mu a bBits b l =
+let mod_exp_fw_mont pbits rLen n mu a bBits b l =
   let aM = M.to_mont pbits rLen n mu a in
-  let resM = mod_exp_mont_precomp_table_ll pbits rLen n mu aM bBits b l in
+  let resM = mod_exp_fw_mont_ pbits rLen n mu aM bBits b l in
   M.from_mont pbits rLen n mu resM
 
 
-val mod_exp_mont_pow2_loop_lemma:
+val mod_exp_pow2_mont_lemma:
     pbits:pos -> rLen:nat
   -> n:pos -> mu:nat
   -> a:nat_mod n
   -> b:nat -> Lemma
   (requires mont_pre pbits rLen n mu)
-  (ensures (let k = mk_nat_mont_group_ll pbits rLen n mu in
-    mod_exp_mont_pow2 pbits rLen n mu a b == LE.exp_pow2 k a b))
+  (ensures
+   (let k = mk_nat_mont_group_ll pbits rLen n mu in
+    let r = mod_exp_pow2_mont pbits rLen n mu a b in
+    r == LE.exp_pow2 k a b /\ r < n))
 
-let rec mod_exp_mont_pow2_loop_lemma pbits rLen n mu a b =
+let rec mod_exp_pow2_mont_lemma pbits rLen n mu a b =
   let k = mk_nat_mont_group_ll pbits rLen n mu in
 
   if b = 0 then begin
@@ -604,26 +642,10 @@ let rec mod_exp_mont_pow2_loop_lemma pbits rLen n mu a b =
   else begin
     Loops.unfold_repeat b (LE.fsqr k) a (b - 1);
     Loops.unfold_repeat b (M.mont_sqr pbits rLen n mu) a (b - 1);
-    mod_exp_mont_pow2_loop_lemma pbits rLen n mu a (b - 1) end
+    mod_exp_pow2_mont_lemma pbits rLen n mu a (b - 1) end
 
 
-val mod_exp_mont_pow2_lemma:
-    pbits:pos -> rLen:nat
-  -> n:pos -> mu:nat
-  -> a:nat_mod n
-  -> b:nat -> Lemma
-  (requires mont_pre pbits rLen n mu)
-  (ensures (let k = mk_nat_mont_group_ll pbits rLen n mu in
-    let r = mod_exp_mont_pow2 pbits rLen n mu a b in
-    r == LE.pow k a (pow2 b) /\ r < n))
-
-let mod_exp_mont_pow2_lemma pbits rLen n mu a b =
-  let k = mk_nat_mont_group_ll pbits rLen n mu in
-  mod_exp_mont_pow2_loop_lemma pbits rLen n mu a b;
-  LE.exp_pow2_lemma k a b
-
-
-val mod_exp_mont_precomp_table_loop_lemma:
+val mod_precomp_table_mont_loop_lemma:
     pbits:pos -> rLen:nat
   -> n:pos -> mu:nat
   -> table_len:Lib.IntTypes.size_nat{1 < table_len}
@@ -635,26 +657,26 @@ val mod_exp_mont_precomp_table_loop_lemma:
     mont_pre pbits rLen n mu /\
     index t01 0 == index t02 0 /\
     index t01 1 == index t02 1)
-  (ensures  (let k = mk_nat_mont_group_ll pbits rLen n mu in
-    let t1 : lseq nat table_len = Loops.repeati j (mod_exp_mont_precomp_table_f pbits rLen n mu a table_len) t01 in
+  (ensures (let k = mk_nat_mont_group_ll pbits rLen n mu in
+    let t1 : lseq nat table_len = Loops.repeati j (mod_precomp_table_mont_f pbits rLen n mu a table_len) t01 in
     let t2 : lseq (nat_mod n) table_len = Loops.repeati j (LE.precomp_table_f k a table_len) t02 in
     (forall (i:nat{i < j + 2}). index t1 i == index t2 i)))
 
-let rec mod_exp_mont_precomp_table_loop_lemma pbits rLen n mu table_len a t01 t02 j =
+let rec mod_precomp_table_mont_loop_lemma pbits rLen n mu table_len a t01 t02 j =
   let k = mk_nat_mont_group_ll pbits rLen n mu in
-  let t1 : lseq nat table_len = Loops.repeati j (mod_exp_mont_precomp_table_f pbits rLen n mu a table_len) t01 in
+  let t1 : lseq nat table_len = Loops.repeati j (mod_precomp_table_mont_f pbits rLen n mu a table_len) t01 in
   let t2 : lseq (nat_mod n) table_len = Loops.repeati j (LE.precomp_table_f k a table_len) t02 in
 
   if j = 0 then begin
-    Loops.eq_repeati0 j (mod_exp_mont_precomp_table_f pbits rLen n mu a table_len) t01;
+    Loops.eq_repeati0 j (mod_precomp_table_mont_f pbits rLen n mu a table_len) t01;
     Loops.eq_repeati0 j (LE.precomp_table_f k a table_len) t02 end
   else begin
-    let t3 : lseq nat table_len = Loops.repeati (j - 1) (mod_exp_mont_precomp_table_f pbits rLen n mu a table_len) t01 in
+    let t3 : lseq nat table_len = Loops.repeati (j - 1) (mod_precomp_table_mont_f pbits rLen n mu a table_len) t01 in
     let t4 : lseq (nat_mod n) table_len = Loops.repeati (j - 1) (LE.precomp_table_f k a table_len) t02 in
 
-    Loops.unfold_repeati j (mod_exp_mont_precomp_table_f pbits rLen n mu a table_len) t01 (j - 1);
+    Loops.unfold_repeati j (mod_precomp_table_mont_f pbits rLen n mu a table_len) t01 (j - 1);
     Loops.unfold_repeati j (LE.precomp_table_f k a table_len) t02 (j - 1);
-    mod_exp_mont_precomp_table_loop_lemma pbits rLen n mu table_len a t01 t02 (j - 1);
+    mod_precomp_table_mont_loop_lemma pbits rLen n mu table_len a t01 t02 (j - 1);
     assert (forall (i:nat{i < j + 1}). index t3 i == index t4 i);
     assert (forall (i:nat{i < j + 1}). index t1 i == index t2 i);
     assert (index t1 (j + 1) == M.mont_mul pbits rLen n mu t3.[j] a);
@@ -664,7 +686,7 @@ let rec mod_exp_mont_precomp_table_loop_lemma pbits rLen n mu table_len a t01 t0
     () end
 
 
-val mod_exp_mont_precomp_table_lemma:
+val mod_precomp_table_mont_lemma:
     pbits:pos -> rLen:nat
   -> n:pos -> mu:nat
   -> table_len:Lib.IntTypes.size_nat{1 < table_len}
@@ -673,187 +695,183 @@ val mod_exp_mont_precomp_table_lemma:
   (requires mont_pre pbits rLen n mu)
   (ensures
    (let k = mk_nat_mont_group_ll pbits rLen n mu in
-    let res = mod_exp_mont_precomp_table pbits rLen n mu table_len a in
-    index res i == LE.pow k a i /\ index res i < n))
+    let t1 = mod_precomp_table_mont pbits rLen n mu table_len a in
+    let t2 = LE.precomp_table k a table_len in
+    index t1 i == index t2 i /\ index t1 i < n))
 
-let mod_exp_mont_precomp_table_lemma pbits rLen n mu table_len a i =
+let mod_precomp_table_mont_lemma pbits rLen n mu table_len a i =
   let k = mk_nat_mont_group_ll pbits rLen n mu in
+
   let res = create table_len 0 in
   let res = res.[0] <- k.LE.one in
   let res = res.[1] <- a in
 
-  let table = create table_len 0 in
-  LE.precomp_table_lemma k a table_len table;
+  let table = create table_len k.LE.one in
   let table = table.[0] <- k.LE.one in
   let table = table.[1] <- a in
-  mod_exp_mont_precomp_table_loop_lemma pbits rLen n mu table_len a res table (table_len - 2);
-  let table1 : lseq (nat_mod n) table_len = Loops.repeati (table_len - 2) (LE.precomp_table_f k a table_len) table in
-  assert (forall (i:nat{i < table_len}). index table1 i == LE.pow k a i);
-  let res1 : lseq nat table_len = Loops.repeati (table_len - 2) (mod_exp_mont_precomp_table_f pbits rLen n mu a table_len) res in
-  assert (forall (i:nat{i < table_len}). index res1 i == index table1 i)
+
+  mod_precomp_table_mont_loop_lemma pbits rLen n mu table_len a res table (table_len - 2)
 
 
-val mod_exp_mont_precomp_ll_f_lemma:
+val mod_exp_fw_mont_f_lemma:
     pbits:pos -> rLen:nat
   -> n:pos -> mu:nat
   -> aM:nat_mod n
   -> bBits:nat -> b:nat{b < pow2 bBits}
   -> l:pos
-  -> table_len:Lib.IntTypes.size_pos{1 < table_len /\ table_len == pow2 l}
-  -> table:lseq nat table_len
-  -> accM0:nat_mod n
-  -> i:nat{i < bBits / l} -> Lemma
-  (requires
-    mont_pre pbits rLen n mu /\
-    table == mod_exp_mont_precomp_table pbits rLen n mu table_len aM)
+  -> table_len:Lib.IntTypes.size_nat{1 < table_len /\ table_len == pow2 l}
+  -> accM:nat_mod n
+  -> i:nat{l * (i + 1) <= bBits} -> Lemma
+  (requires mont_pre pbits rLen n mu)
   (ensures
-    (let k = mk_nat_mont_group_ll pbits rLen n mu in
-     mod_exp_mont_precomp_f_ll pbits rLen n mu bBits b l table_len table i accM0 ==
-     LE.exp_precomp_f k aM bBits b l i accM0))
+   (let k = mk_nat_mont_group_ll pbits rLen n mu in
+    let t1 = mod_precomp_table_mont pbits rLen n mu table_len aM in
+    let t2 = LE.precomp_table k aM table_len in
+    let r = mod_exp_fw_mont_f pbits rLen n mu bBits b l table_len t1 i accM in
+    r == LE.exp_fw_f k bBits b l table_len t2 i accM /\ r < n))
 
-let mod_exp_mont_precomp_ll_f_lemma pbits rLen n mu aM bBits b l table_len table accM0 i =
+let mod_exp_fw_mont_f_lemma pbits rLen n mu aM bBits b l table_len accM i =
   let k = mk_nat_mont_group_ll pbits rLen n mu in
-  let accM1 = mod_exp_mont_precomp_f_ll pbits rLen n mu bBits b l table_len table i accM0 in
-  let lbits = b / pow2 (bBits - l * i - l) % table_len in
-  let acc_pow2l = mod_exp_mont_pow2 pbits rLen n mu accM0 l in // pow k acc (pow2 l)
-  mod_exp_mont_precomp_table_lemma pbits rLen n mu table_len aM lbits;
-  assert (index table lbits == LE.pow k aM lbits);
-  mod_exp_mont_pow2_lemma pbits rLen n mu accM0 l;
-  assert (mod_exp_mont_pow2 pbits rLen n mu accM0 l == LE.pow k accM0 (pow2 l));
-  assert (accM1 == M.mont_mul pbits rLen n mu (LE.pow k accM0 table_len) (LE.pow k aM lbits))
+  let t1 = mod_precomp_table_mont pbits rLen n mu table_len aM in
+  let t2 = LE.precomp_table k aM table_len in
+
+  let bits_l = b / pow2 (bBits - l * i - l) % table_len in
+  mod_precomp_table_mont_lemma pbits rLen n mu table_len aM bits_l;
+  assert (index t1 bits_l == index t2 bits_l);
+  mod_exp_pow2_mont_lemma pbits rLen n mu accM l
 
 
-val mod_exp_mont_precomp_ll_rem_lemma:
+val mod_exp_fw_mont_rem_lemma:
     pbits:pos -> rLen:nat
   -> n:pos -> mu:nat
   -> aM:nat_mod n
   -> bBits:nat -> b:nat{b < pow2 bBits}
   -> l:pos
-  -> table_len:Lib.IntTypes.size_pos{1 < table_len /\ table_len == pow2 l}
-  -> table:lseq nat table_len
+  -> table_len:Lib.IntTypes.size_nat{1 < table_len /\ table_len == pow2 l}
   -> accM:nat_mod n -> Lemma
-  (requires
-    mont_pre pbits rLen n mu /\
-    table == mod_exp_mont_precomp_table pbits rLen n mu table_len aM)
+  (requires mont_pre pbits rLen n mu)
   (ensures
-    (let k = mk_nat_mont_group_ll pbits rLen n mu in let c = bBits % l in
-     let r = mod_exp_mont_precomp_rem_ll pbits rLen n mu bBits b l table_len table accM in
-     r == k.LE.fmul (LE.pow k accM (pow2 c)) (LE.pow k aM (b % pow2 c)) /\ r < n))
+   (let k = mk_nat_mont_group_ll pbits rLen n mu in
+    let t1 = mod_precomp_table_mont pbits rLen n mu table_len aM in
+    let t2 = LE.precomp_table k aM table_len in
+    let r = mod_exp_fw_mont_rem pbits rLen n mu bBits b l table_len t1 accM in
+    r == LE.exp_fw_rem k bBits b l table_len t2 accM /\ r < n))
 
-let mod_exp_mont_precomp_ll_rem_lemma pbits rLen n mu aM bBits b l table_len table accM =
+let mod_exp_fw_mont_rem_lemma pbits rLen n mu aM bBits b l table_len accM =
   let k = mk_nat_mont_group_ll pbits rLen n mu in
-  let accM1 = mod_exp_mont_precomp_rem_ll pbits rLen n mu bBits b l table_len table accM in
+  let t1 = mod_precomp_table_mont pbits rLen n mu table_len aM in
+  let t2 = LE.precomp_table k aM table_len in
 
   let c = bBits % l in
   let bits_c = b % pow2 c in
-  let acc_pow2c = mod_exp_mont_pow2 pbits rLen n mu accM c in // pow k acc (pow2 c)
   Math.Lemmas.pow2_lt_compat l c;
-  let a_powbits_c = table.[bits_c] in //select_table // pow k a bits_c
-  mod_exp_mont_precomp_table_lemma pbits rLen n mu table_len aM bits_c;
-  mod_exp_mont_pow2_lemma pbits rLen n mu accM c
+
+  mod_precomp_table_mont_lemma pbits rLen n mu table_len aM bits_c;
+  assert (index t1 bits_c == index t2 bits_c);
+  mod_exp_pow2_mont_lemma pbits rLen n mu accM c
 
 
-#push-options "--z3rlimit 150"
-val mod_exp_mont_precomp_ll_loop_lemma:
+val mod_exp_fw_mont_loop_lemma:
     pbits:pos -> rLen:nat
   -> n:pos -> mu:nat
   -> aM:nat_mod n
   -> bBits:nat -> b:nat{b < pow2 bBits}
   -> l:pos
   -> table_len:Lib.IntTypes.size_pos{1 < table_len /\ table_len == pow2 l}
-  -> table:lseq nat table_len
   -> accM0:nat_mod n
-  -> i:nat{i <= bBits / l} -> Lemma
-  (requires
-    mont_pre pbits rLen n mu /\
-    table == mod_exp_mont_precomp_table pbits rLen n mu table_len aM)
+  -> j:nat{l * j <= bBits } -> Lemma
+  (requires mont_pre pbits rLen n mu)
   (ensures
-    (let k = mk_nat_mont_group_ll pbits rLen n mu in
-     let accM1 = Loops.repeati i (mod_exp_mont_precomp_f_ll pbits rLen n mu bBits b l table_len table) accM0 in
-     let accM2 : nat_mod n = Loops.repeati i (LE.exp_precomp_f k aM bBits b l) accM0 in
-     accM1 == accM2 /\ accM1 < n))
+   (let k = mk_nat_mont_group_ll pbits rLen n mu in
+    let t1 = mod_precomp_table_mont pbits rLen n mu table_len aM in
+    let t2 = LE.precomp_table k aM table_len in
 
-let rec mod_exp_mont_precomp_ll_loop_lemma pbits rLen n mu aM bBits b l table_len table accM0 i =
-  Math.Lemmas.lemma_mult_le_left l i (bBits / l);
+    let accM1 = Loops.repeati j (mod_exp_fw_mont_f pbits rLen n mu bBits b l table_len t1) accM0 in
+    let accM2 : nat_mod n = Loops.repeati j (LE.exp_fw_f k bBits b l table_len t2) accM0 in
+    accM1 == accM2 /\ accM1 < n))
+
+let rec mod_exp_fw_mont_loop_lemma pbits rLen n mu aM bBits b l table_len accM0 j =
   let k = mk_nat_mont_group_ll pbits rLen n mu in
-  //let accM1 = Loops.repeati i (mod_exp_mont_precomp_f_ll pbits rLen n mu bBits b l table_len table) accM0 in
-  //let accM2 : nat_mod n = Loops.repeati i (LE.exp_precomp_f k aM bBits b l) accM0 in
+  let t1 = mod_precomp_table_mont pbits rLen n mu table_len aM in
+  let t2 = LE.precomp_table k aM table_len in
 
-  if i = 0 then begin
-    Loops.eq_repeati0 i (mod_exp_mont_precomp_f_ll pbits rLen n mu bBits b l table_len table) accM0;
-    Loops.eq_repeati0 i (LE.exp_precomp_f k aM bBits b l) accM0 end
+  if j = 0 then begin
+    Loops.eq_repeati0 j (mod_exp_fw_mont_f pbits rLen n mu bBits b l table_len t1) accM0;
+    Loops.eq_repeati0 j (LE.exp_fw_f k bBits b l table_len t2) accM0 end
   else begin
-    mod_exp_mont_precomp_ll_loop_lemma pbits rLen n mu aM bBits b l table_len table accM0 (i - 1);
-    //let accM3 = Loops.repeati (i - 1) (mod_exp_mont_precomp_f_ll pbits rLen n mu bBits b l table_len table) accM0 in
-    let accM4 : nat_mod n = Loops.repeati (i - 1) (LE.exp_precomp_f k aM bBits b l) accM0 in
-    Loops.unfold_repeati i (LE.exp_precomp_f k aM bBits b l) accM0 (i - 1);
-    Loops.unfold_repeati i (mod_exp_mont_precomp_f_ll pbits rLen n mu bBits b l table_len table) accM0 (i - 1);
-    //assert (accM1 == mod_exp_mont_precomp_f_ll pbits rLen n mu bBits b l table_len table (i - 1) accM3);
-    //assert (accM2 == LE.exp_precomp_f k aM bBits b l (i - 1) accM4);
-    //assert (accM3 == accM4 /\ accM3 < n);
-    mod_exp_mont_precomp_ll_f_lemma pbits rLen n mu aM bBits b l table_len table accM4 (i - 1);
+    Math.Lemmas.lemma_mult_lt_left l (j - 1) j;
+    let accM4 = Loops.repeati (j - 1) (LE.exp_fw_f k bBits b l table_len t2) accM0 in
+    Loops.unfold_repeati j (LE.exp_fw_f k bBits b l table_len t2) accM0 (j - 1);
+    Loops.unfold_repeati j (mod_exp_fw_mont_f pbits rLen n mu bBits b l table_len t1) accM0 (j - 1);
+    mod_exp_fw_mont_loop_lemma pbits rLen n mu aM bBits b l table_len accM0 (j - 1);
+    mod_exp_fw_mont_f_lemma pbits rLen n mu aM bBits b l table_len accM4 (j - 1);
     () end
-#pop-options
 
 
-val mod_exp_mont_precomp_table_ll_lemma:
+val mod_exp_fw_mont_aux_lemma:
     pbits:pos -> rLen:pos
   -> n:pos -> mu:nat
   -> aM:nat_mod n
   -> bBits:nat -> b:nat{b < pow2 bBits}
   -> l:pos{pow2 l <= Lib.IntTypes.max_size_t} -> Lemma
   (requires mont_pre pbits rLen n mu)
-  (ensures  (let k = mk_nat_mont_group_ll pbits rLen n mu in
-    let acc = LE.exp_precomp k aM bBits b l in let c = bBits % l in
-    let res_s = k.LE.fmul (LE.pow k acc (pow2 c)) (LE.pow k aM (b % pow2 c)) in
-    let res = mod_exp_mont_precomp_table_ll pbits rLen n mu aM bBits b l in
-    res == res_s /\ res < n /\ res_s == LE.pow k aM b))
+  (ensures
+   (let k = mk_nat_mont_group_ll pbits rLen n mu in
+    let r = mod_exp_fw_mont_ pbits rLen n mu aM bBits b l in
+    r == LE.exp_fw k aM bBits b l /\ r < n))
 
-let mod_exp_mont_precomp_table_ll_lemma pbits rLen n mu aM bBits b l =
+let mod_exp_fw_mont_aux_lemma pbits rLen n mu aM bBits b l =
   let r = pow2 (pbits * rLen) in
   let d, k = M.eea_pow2_odd (pbits * rLen) n in
   M.mont_preconditions_d pbits rLen n;
-
   let k1 = mk_nat_mont_group_ll pbits rLen n mu in
+
   let oneM = M.to_mont pbits rLen n mu 1 in
   M.to_mont_lemma pbits rLen n d mu 1;
   assert (oneM == 1 * r % n);
 
-  let table_len = pow2 l in
   Math.Lemmas.pow2_le_compat l 1;
-  let table = mod_exp_mont_precomp_table pbits rLen n mu table_len aM in
-  let accM : nat = Loops.repeati (bBits / l) (mod_exp_mont_precomp_f_ll pbits rLen n mu bBits b l table_len table) oneM in
-  mod_exp_mont_precomp_ll_loop_lemma pbits rLen n mu aM bBits b l table_len table oneM (bBits / l);
-  mod_exp_mont_precomp_ll_rem_lemma pbits rLen n mu aM bBits b l table_len table accM;
-  LE.exp_precomp_lemma1 k1 aM bBits b l
+  let table_len = pow2 l in
+  assert (1 < table_len /\ table_len <= Lib.IntTypes.max_size_t);
+  let t1 = mod_precomp_table_mont pbits rLen n mu table_len aM in
+  let t2 = LE.precomp_table k1 aM table_len in
+
+  //Math.Lemmas.multiply_fractions bBits l;
+  let accM : nat = Loops.repeati (bBits / l) (mod_exp_fw_mont_f pbits rLen n mu bBits b l table_len t1) oneM in
+  mod_exp_fw_mont_loop_lemma pbits rLen n mu aM bBits b l table_len oneM (bBits / l);
+  assert (accM < n);
+  mod_exp_fw_mont_rem_lemma pbits rLen n mu aM bBits b l table_len accM
 
 
-val mod_exp_mont_precomp_ll_lemma:
+val mod_exp_fw_mont_lemma:
     pbits:pos -> rLen:nat
   -> n:pos -> mu:nat
   -> a:nat_mod n
   -> bBits:nat -> b:pos{b < pow2 bBits}
   -> l:pos{pow2 l <= Lib.IntTypes.max_size_t} -> Lemma
   (requires mont_pre pbits rLen n mu)
-  (ensures  mod_exp_mont_precomp_ll pbits rLen n mu a bBits b l == pow_mod #n a b)
+  (ensures  mod_exp_fw_mont pbits rLen n mu a bBits b l == pow_mod #n a b)
 
-let mod_exp_mont_precomp_ll_lemma pbits rLen n mu a bBits b l =
+let mod_exp_fw_mont_lemma pbits rLen n mu a bBits b l =
   let r = pow2 (pbits * rLen) in
   let d, k = M.eea_pow2_odd (pbits * rLen) n in
   M.mont_preconditions_d pbits rLen n;
-
-  let k0 = mk_nat_mont_group n r d in
   let k1 = mk_nat_mont_group_ll pbits rLen n mu in
 
   let aM = M.to_mont pbits rLen n mu a in
   M.to_mont_lemma pbits rLen n d mu a;
   assert (aM == a * r % n);
 
-  let resM = mod_exp_mont_precomp_table_ll pbits rLen n mu aM bBits b l in
-  mod_exp_mont_precomp_table_ll_lemma pbits rLen n mu aM bBits b l;
+  let resM = mod_exp_fw_mont_ pbits rLen n mu aM bBits b l in
+  mod_exp_fw_mont_aux_lemma pbits rLen n mu aM bBits b l;
+  assert (resM == LE.exp_fw k1 aM bBits b l);
+  LE.exp_fw_lemma k1 aM bBits b l;
   assert (resM == LE.pow k1 aM b);
-  pow_nat_mont_ll_is_pow_nat_mont pbits rLen n mu aM b;
+
   let res = M.from_mont pbits rLen n mu resM in
   M.from_mont_lemma pbits rLen n d mu resM;
-  mont_mod_exp_lemma n r d a b;
+  assert (res == resM * d % n);
+
+  mod_exp_mont_ll_lemma pbits rLen n mu a b;
+  assert (res == pow a b % n);
   lemma_pow_mod #n a b
